WIP

src/pf2ir/FutureCertify.v
@@ -24,10 +24,9 @@ Require Import Global.
 Require Import Local.
 Require Import Thread.
 
-Require Import PFCertify.
+Require Import PFConsistent.
 
 Set Implicit Arguments.
-Set Nested Proofs Allowed.
 
 
 Module FutureCertify.
@@ -2200,4 +2199,391 @@ Module FutureCertify.
       i. des.
       esplits; [econs 10|..]; eauto. econs; ss.
   Qed.
+
+
+  Section FutureCertify.
+    Variable lang: language.
+
+    Variant certify (reserved: TimeMap.t) (loc: Loc.t) (ts: Time.t) (th: Thread.t lang): Prop :=
+      | certify_failure
+          pf e th1 th2
+          (STEPS: rtc (pstep (Thread.step reserved true) (strict_pf /1\ ThreadEvent.is_silent))
+                      th th1)
+          (STEP_FAILURE: Thread.step reserved pf e th1 th2)
+          (EVENT_FAILURE: ThreadEvent.get_machine_event e = MachineEvent.failure)
+          (EVENT_PF: strict_pf e)
+      | certify_fulfill
+          pf e th1 th2
+          from to val released ord
+          (STEPS: rtc (pstep (Thread.step reserved true) (strict_pf /1\ ThreadEvent.is_silent))
+                      th th1)
+          (STEP_FULFILL: Thread.step reserved pf e th1 th2)
+          (EVENT_FULFILL: ThreadEvent.is_writing e = Some (loc, from, to, val, released, ord))
+          (TO: Time.lt ts to)
+          (ORD: Ordering.le ord Ordering.na)
+    .
+
+    Lemma spf_consistent_certify
+          th loc
+          (LC_WF: Local.wf (Thread.local th) (Thread.global th))
+          (GL_WF: Global.wf (Thread.global th))
+          (CONS: PFConsistent.spf_consistent th)
+          (PROMISED: Local.promises (Thread.local th) loc = true):
+      certify (Memory.max_timemap (Global.memory (Thread.global th)))
+              loc (Memory.max_ts loc (Global.memory (Thread.global th)))
+              (Thread.fully_reserved th).
+    Proof.
+      inv CONS.
+      { econs 1; eauto. }
+      exploit (Memory.max_ts_spec loc); try apply GL_WF. i. des.
+      remember (Memory.max_ts loc (Global.memory (Thread.global th))) as ts in *.
+      exploit Thread.fully_reserved_wf; eauto.
+      clear LC_WF GL_WF. i. des.
+      remember (Memory.max_timemap (Global.memory (Thread.global th))) as reserved.
+      remember (Thread.fully_reserved th) as th0.
+      replace (Local.promises (Thread.local th) loc) with
+        (Local.promises (Thread.local th0) loc) in * by (subst; ss).
+      replace (Global.memory (Thread.global th)) with
+        (Global.memory (Thread.global th0)) in * by (subst; ss).
+      clear th Heqts Heqreserved Heqth0 MAX. revert PROMISED.
+      induction STEPS; i.
+      { rewrite PROMISES in *. ss. }
+      destruct (Local.promises (Thread.local y) loc) eqn:PROMISEDY.
+      { dup H. inv H0.
+        exploit Thread.step_future; try exact STEP; eauto. i. des.
+        exploit Memory.future_get1; try apply GL_FUTURE; eauto. i. des.
+        exploit IHSTEPS; eauto. i. inv x2.
+        - econs 1; try exact STEP_FAILURE; eauto.
+        - econs 2; try exact STEP_FULFILL; eauto.
+      }
+
+      move PROMISEDY at bottom.
+      inv H. inv STEP.
+      inv STEP0; ss; (try congr); (try by inv LOCAL; ss; congr).
+      { (* write *)
+        assert (loc0 = loc /\ Ordering.le ord Ordering.na).
+        { inv LOCAL. inv FULFILL; ss; try congr. split; ss.
+          revert PROMISEDY. erewrite BoolMap.remove_o; eauto.
+          condtac; ss. congr.
+        }
+        des. subst.
+        destruct (TimeFacts.le_lt_dec to (Memory.max_ts loc (Global.memory gl1))); cycle 1.
+        { econs 2; [refl|..].
+          - econs 2; [|econs 3]; eauto.
+          - ss.
+          - exploit Memory.max_ts_spec; try exact GET. i. des.
+            eapply TimeFacts.le_lt_lt; eauto.
+          - ss.
+        }
+        exploit (Memory.max_ts_spec loc); try apply GL_WF. i. des.
+        destruct msg0. clear MAX.
+        econs 1; [refl|..].
+        - econs 2; [|econs 9]; eauto.
+          econs. econs 2; try exact GET0.
+          + unfold TView.racy_view.
+            eapply TimeFacts.lt_le_lt; eauto.
+            inv LOCAL. inv WRITABLE. ss.
+            eapply TimeFacts.le_lt_lt; eauto.
+            apply LC_WF.
+          + destruct ord; ss.
+        - ss.
+        - ss.
+      }
+
+      { (* update *)
+        assert (Ordering.le ordw Ordering.na).
+        { inv LOCAL1. inv LOCAL2.  inv FULFILL; ss; try congr. }
+        econs 1; [refl|..].
+        - econs 2; [|econs 10]; eauto.
+        - ss.
+        - ii. ss. des. destruct ordw; ss.
+      }
+    Qed.
+
+    Variant thread_map (f: map_t) (reserved: TimeMap.t) (th fth: Thread.t lang): Prop :=
+      | thread_map_intro
+          (STATE: Thread.state th = Thread.state fth)
+          (LOCAL: local_map f (Thread.local th) (Thread.local fth))
+          (GLOBAL: global_map f reserved (Local.reserves (Thread.local th))
+                              (Thread.global th) (Thread.global fth))
+          (FPROMISES: Local.promises (Thread.local fth) = BoolMap.bot)
+          (GRESERVES: Global.reserves (Thread.global th) = BoolMap.top)
+          (FGRESERVES: Global.reserves (Thread.global fth) = BoolMap.bot)
+    .
+
+    Lemma event_map_program_event
+          f e fe
+          (MAP: event_map f e fe):
+      ThreadEvent.get_program_event e = ThreadEvent.get_program_event fe.
+    Proof.
+      inv MAP; ss.
+    Qed.
+
+    Lemma event_map_machine_event
+          f e fe
+          (MAP: event_map f e fe):
+      ThreadEvent.get_machine_event e = ThreadEvent.get_machine_event fe.
+    Proof.
+      inv MAP; ss.
+    Qed.
+
+    Lemma event_map_strict_pf
+          f e fe
+          (MAP: event_map f e fe):
+      strict_pf e <-> strict_pf fe.
+    Proof.
+      inv MAP; ss.
+      - destruct to, fto; ss.
+      - destruct to, fto; ss.
+      - destruct to, fto; ss.
+    Qed.
+
+    Lemma event_map_is_silent
+          f e fe
+          (MAP: event_map f e fe):
+      ThreadEvent.is_silent e <-> ThreadEvent.is_silent fe.
+    Proof.
+      inv MAP; ss.
+    Qed.
+
+    Lemma map_step
+          reserved freserved
+          f1 th1 fth1
+          e th2
+          (MAP_WF1: map_wf f1)
+          (MAP_COMPLETE1: map_complete
+                            f1
+                            (Global.memory (Thread.global th1))
+                            (Global.memory (Thread.global fth1)))
+          (MAP1: thread_map f1 reserved th1 fth1)
+          (LC_WF1: Local.wf (Thread.local th1) (Thread.global th1))
+          (GL_WF1: Global.wf (Thread.global th1))
+          (FLC_WF1: Local.wf (Thread.local fth1) (Thread.global fth1))
+          (FGL_WF1: Global.wf (Thread.global fth1))
+          (RESERVED: Memory.closed_timemap reserved (Global.memory (Thread.global th1)))
+          (STEP: Thread.step reserved true e th1 th2)
+          (EVENT: ~ ThreadEvent.is_racy_promise e):
+      exists f2 fe fth2,
+        (<<FSTEP: Thread.step freserved true fe fth1 fth2>>) /\
+        (<<EVENT: event_map f2 e fe>>) /\
+        (<<MAP_INCR: f1 <3= f2>>) /\
+        (<<MAP_WF2: map_wf f2>>) /\
+        (<<MAP_COMPLETE2: map_complete
+                            f2
+                            (Global.memory (Thread.global th2))
+                            (Global.memory (Thread.global fth2))>>) /\
+        (<<MAP2: thread_map f2 reserved th2 fth2>>).
+    Proof.
+      destruct th1, fth1. inv MAP1. ss. subst. inv STEP.
+      exploit map_program_step; try exact LOCAL; try exact GLOBAL; eauto. i. des.
+      esplits; eauto.
+      - econs; try exact FSTEP.
+        erewrite <- event_map_program_event; eauto.
+      - eauto.
+      - exploit Local.program_step_reserves; try exact STEP0. i. des.
+        exploit Local.program_step_promises; try exact FSTEP. i. des.
+        exploit Local.program_step_reserves; try exact FSTEP. i. des.
+        econs; eauto; s; try congr.
+        apply BoolMap.antisym; try apply BoolMap.bot_spec.
+        etrans; eauto. rewrite FPROMISES. refl.
+    Qed.
+
+    Lemma map_rtc_step
+          reserved freserved
+          f1 th1 fth1
+          th2
+          (MAP_WF1: map_wf f1)
+          (MAP_COMPLETE1: map_complete
+                            f1
+                            (Global.memory (Thread.global th1))
+                            (Global.memory (Thread.global fth1)))
+          (MAP1: thread_map f1 reserved th1 fth1)
+          (LC_WF1: Local.wf (Thread.local th1) (Thread.global th1))
+          (GL_WF1: Global.wf (Thread.global th1))
+          (FLC_WF1: Local.wf (Thread.local fth1) (Thread.global fth1))
+          (FGL_WF1: Global.wf (Thread.global fth1))
+          (RESERVED: Memory.closed_timemap reserved (Global.memory (Thread.global th1)))
+          (STEPS: rtc (pstep (Thread.step reserved true) (strict_pf /1\ ThreadEvent.is_silent)) th1 th2):
+      exists f2 fth2,
+        (<<FSTEPS: rtc (pstep (Thread.step freserved true) (strict_pf /1\ ThreadEvent.is_silent)) fth1 fth2>>) /\
+        (<<MAP_INCR: f1 <3= f2>>) /\
+        (<<MAP_WF2: map_wf f2>>) /\
+        (<<MAP_COMPLETE2: map_complete
+                            f2
+                            (Global.memory (Thread.global th2))
+                            (Global.memory (Thread.global fth2))>>) /\
+        (<<MAP2: thread_map f2 reserved th2 fth2>>).
+    Proof.
+      revert f1 fth1 MAP_WF1 MAP_COMPLETE1 MAP1 FLC_WF1 FGL_WF1.
+      induction STEPS; i.
+      { esplits; eauto. }
+      inv H. des.
+      exploit map_step; eauto. i. des.
+      exploit Thread.step_future; try exact STEP; eauto. i. des.
+      exploit Thread.step_future; try exact FSTEP; eauto. i. des.
+      hexploit Memory.future_closed_timemap; try apply GL_FUTURE; eauto. i.
+      exploit IHSTEPS; eauto. i. des.
+      esplits; try exact MAP0; eauto.
+      econs 2; try exact FSTEPS.
+      econs; eauto.
+      erewrite <- event_map_strict_pf; eauto.
+      erewrite <- event_map_is_silent; eauto.
+    Qed.
+
+    Lemma event_map_is_writing
+          f e fe
+          loc from to val released ord
+          (MAP: event_map f e fe)
+          (WRITING: ThreadEvent.is_writing e = Some (loc, from, to, val, released, ord)):
+      exists ffrom fto freleased,
+        (<<FWRITING: ThreadEvent.is_writing fe = Some (loc, ffrom, fto, val, freleased, ord)>>) /\
+        (<<FROM: f loc from ffrom>>) /\
+        (<<TO: f loc to fto>>) /\
+        (<<RELEASED: opt_view_map f released freleased>>).
+    Proof.
+      inv MAP; ss; inv WRITING; esplits; eauto.
+    Qed.
+
+    Lemma map_certify
+          reserved freserved
+          f th fth
+          loc ts fts
+          (MAP_WF: map_wf f)
+          (MAP_COMPLETE: map_complete
+                           f
+                           (Global.memory (Thread.global th))
+                           (Global.memory (Thread.global fth)))
+          (MAP: thread_map f reserved th fth)
+          (LC_WF: Local.wf (Thread.local th) (Thread.global th))
+          (GL_WF: Global.wf (Thread.global th))
+          (FLC_WF: Local.wf (Thread.local fth) (Thread.global fth))
+          (FGL_WF: Global.wf (Thread.global fth))
+          (RESERVED: Memory.closed_timemap reserved (Global.memory (Thread.global th)))
+          (TS: f loc ts fts)
+          (CERTIFY: certify reserved loc ts th):
+      certify freserved loc fts fth.
+    Proof.
+      inv CERTIFY.
+      { exploit map_rtc_step; try exact STEPS; eauto. i. des.
+        exploit Thread.rtc_all_step_future; try eapply rtc_implies; try exact STEPS; eauto.
+        { i. inv H. econs. econs. eauto. }
+        i. des.
+        exploit Thread.rtc_all_step_future; try eapply rtc_implies; try exact FSTEPS; eauto.
+        { i. inv H. econs. econs. eauto. }
+        i. des.
+        hexploit Memory.future_closed_timemap; try apply GL_FUTURE; eauto. i.
+        destruct pf; try by (inv STEP_FAILURE; inv STEP; ss).
+        exploit map_step; try exact STEP_FAILURE; try exact MAP2; eauto. i. des.
+        econs 1; try exact FSTEP; eauto.
+        - erewrite <- event_map_machine_event; eauto.
+        - erewrite <- event_map_strict_pf; eauto.
+      }
+      { exploit map_rtc_step; try exact STEPS; eauto.
+        instantiate (1:=freserved). i. des.
+        exploit Thread.rtc_all_step_future; try eapply rtc_implies; try exact STEPS; eauto.
+        { i. inv H. econs. econs. eauto. }
+        i. des.
+        exploit Thread.rtc_all_step_future; try eapply rtc_implies; try exact FSTEPS; eauto.
+        { i. inv H. econs. econs. eauto. }
+        i. des.
+        hexploit Memory.future_closed_timemap; try apply GL_FUTURE; eauto. i.
+        destruct pf; try by (inv STEP_FULFILL; inv STEP; ss).
+        exploit map_step; try exact STEP_FULFILL; try exact MAP2; eauto.
+        { destruct e; ss. }
+        instantiate (1:=freserved). i. des.
+        exploit event_map_is_writing; try exact EVENT; eauto. i. des.
+        econs 2; try exact FSTEP; eauto.
+        inv MAP_WF0. eapply MAP_LT; try exact TO; eauto.
+      }
+    Qed.
+
+    Lemma future_reserved_spaced
+          loc mem fmem
+          (INHABITED: Memory.inhabited mem)
+          (FUTURE: Memory.future mem fmem)
+          (RESERVED: forall ffrom fto fmsg
+                       (GET: Memory.get loc fto mem = None)
+                       (FGET: Memory.get loc fto fmem = Some (ffrom, fmsg)),
+              Time.lt (Memory.max_ts loc mem) ffrom):
+      exists max,
+        Time.lt (Memory.max_ts loc mem) max /\
+        forall ffrom fto fmsg
+          (GET: Memory.get loc fto mem = None)
+          (FGET: Memory.get loc fto fmem = Some (ffrom, fmsg)),
+          Time.lt max ffrom.
+    Proof.
+      destruct (TimeFacts.le_lt_dec (Memory.max_ts loc fmem) (Memory.max_ts loc mem)).
+      { exists (Time.incr (Memory.max_ts loc mem)).
+        split; try apply Time.incr_spec. i.
+        exploit RESERVED; eauto. i.
+        exploit Memory.get_ts; try exact FGET. i. des; timetac.
+        exploit Memory.max_ts_spec; try exact FGET. i. des.
+        rewrite x1 in x0. rewrite l in MAX. timetac.
+      }
+      exploit (Memory.max_ts_spec loc); try apply INHABITED. i. des. clear MAX.
+      exploit Memory.future_get1; try exact FUTURE; eauto. i. des.
+      exploit Memory.next_exists; try exact x0; try exact l. i. des.
+      exploit RESERVED; try exact x1.
+      { destruct (Memory.get loc to mem) as [[]|] eqn:X; ss.
+        exploit Memory.max_ts_spec; try exact X. i. des. timetac.
+      }
+      i.
+      exists (Time.middle (Memory.max_ts loc mem) from0).
+      split; try apply Time.middle_spec; ss. i.
+      exploit RESERVED; try exact FGET; eauto. i.
+      destruct (TimeFacts.le_lt_dec to fto).
+      { inv l0.
+        - exploit Memory.lt_get; try exact H; eauto. i.
+          eapply TimeFacts.lt_le_lt; try exact x6.
+          eapply TimeFacts.lt_le_lt; [apply Time.middle_spec; ss|].
+          exploit Memory.get_ts; try exact x1. i. des; timetac. econs. ss.
+        - inv H. rewrite x1 in *. inv FGET.
+          apply Time.middle_spec; ss.
+      }
+      exploit (x3 fto); try congr.
+      eapply TimeFacts.lt_le_lt; try exact x5.
+      exploit Memory.get_ts; try exact FGET. i. des; timetac. econs. ss.
+    Qed.
+
+    Lemma future_map
+          rsv mem fmem
+          (INHABITED: Memory.inhabited mem)
+          (FUTURE: Memory.future mem fmem)
+          (RESERVED: forall loc ffrom fto fmsg
+                       (RESERVED: rsv loc = true)
+                       (GET: Memory.get loc fto mem = None)
+                       (FGET: Memory.get loc fto fmem = Some (ffrom, fmsg)),
+              Time.lt (Memory.max_ts loc mem) ffrom):
+      exists f,
+        (<<MAP_WF: map_wf f>>) /\
+        (<<MAP_COMPLETE: map_complete f mem fmem>>) /\
+        (<<MAP: memory_map f (Memory.max_timemap mem) rsv mem fmem>>).
+    Proof.
+      exists (fun loc ts fts =>
+           ts = fts /\
+           exists from to msg,
+             Memory.get loc to mem = Some (from, msg) /\ (ts = from \/ ts = to)).
+      splits.
+      { econs; ii; try by (des; subst; ss).
+        splits; ss. esplits; eauto.
+      }
+      { ii. des; subst.
+        - exploit Memory.future_get1; try exact FUTURE; eauto. i. des.
+          esplits; eauto. left. ss.
+        - exploit Memory.future_get1; try exact FUTURE; eauto. i. des.
+          esplits; eauto. right. ss.
+      }
+
+      ii. destruct (rsv loc) eqn:RSV.
+      { exploit (future_reserved_spaced loc); eauto. i. des.
+        econs; i.
+        - instantiate (1:=max).
+          exploit Memory.future_get1; try exact FUTURE; eauto. i. des.
+          admit.
+        - admit.
+      }
+      { admit.
+      }
+    Admitted.
+  End FutureCertify.
 End FutureCertify.
